Add some progress on the Lindenbaum Lemma

Fine/Completeness/Lindenbaum.lean
@@ -1,21 +1,67 @@
 import Fine.FormalTheories
+import Mathlib.Data.Prod.Lex
 
 open Classical
 
-def lindenbaumSequence (t : Th) (Δ : Ctx) : Nat → Nat → Ctx
-  | 0, 0 => t.val
-  | i + 1, 0 => { f : Form | ∃j : Nat, f ∈ lindenbaumSequence t Δ i j }
-  | i, j + 1 => 
-    have prev := lindenbaumSequence t Δ i j
+def lindenbaumSequence (t : Th) (Δ : Ctx) : Lex (Nat × Nat) → Ctx
+  | ⟨0, 0⟩ => t.val
+  | ⟨i + 1, 0⟩ => { f : Form | ∃j : Nat, f ∈ lindenbaumSequence t Δ ⟨i, j⟩ }
+  | ⟨i, j + 1⟩ => 
+    have prev := lindenbaumSequence t Δ ⟨i, j⟩
     have ⟨l,r⟩ := Denumerable.ofNat (Form × Form) j
     if l ¦ r ∈ ▲prev 
     then if ▲(prev ∪ {l}) ∩ Δ = ∅
       then prev ∪ {l}
       else prev ∪ {r}
     else prev
-  termination_by lindenbaumSequence t Δ i j => (i,j)
+  termination_by lindenbaumSequence t Δ p => (p.fst, p.snd)
 
-def lindenbaumExtension (t : Th) (Δ : Ctx) : Ctx := {f | ∃n m : Nat, f ∈ lindenbaumSequence t Δ n m }
+lemma lindenbaumSequenceMonotone { t : Th } { Δ : Ctx } : ∀b a, a ≤ b → lindenbaumSequence t Δ a ⊆ lindenbaumSequence t Δ b := by
+  intros b
+  match b with
+    | ⟨0, 0⟩ => 
+      intros a h₁
+      cases h₁
+      case left a₁ _ h₂ => exact False.elim $ Nat.not_lt_zero a₁ h₂
+      case right b₁ h₂ =>
+        rw [Nat.le_zero_eq b₁] at h₂
+        rw [h₂]
+    | ⟨i + 1, 0⟩ => 
+      intros a h₁
+      cases h₁
+      case left a₁ b₁ h₂ => 
+        have l₁ : a₁ < i ∨ a₁ = i := Nat.lt_or_eq_of_le $ Nat.lt_succ.mp h₂
+        have l₂ : a₁ < i ∨ a₁ = i ∧ b₁ ≤ b₁ := by 
+          cases l₁
+          case inl h₂ => exact Or.inl h₂
+          case inr h₂ => exact Or.inr ⟨h₂, le_refl b₁⟩
+        have l₃ := (Prod.Lex.le_iff (a₁, b₁) (i,b₁)).mpr l₂
+        have l₄ := @lindenbaumSequenceMonotone t Δ (i,b₁) (a₁, b₁) l₃
+        apply le_trans l₄
+        intros f h₂
+        exact ⟨b₁,h₂⟩
+      case right b₁ h₂ => 
+        rw [Nat.le_zero_eq b₁] at h₂
+        rw [h₂]
+    | ⟨i, j + 1⟩ => 
+      intros a h₁
+      cases h₁
+      case left a₁ b₁ h₂ => sorry
+      case right b₁ h₂ => 
+        cases h₂
+        case refl => intros f h₁; assumption
+        case step h₂ => 
+          have l₁ : i < i ∨ i = i ∧ b₁ ≤ j := Or.inr ⟨rfl, h₂⟩
+          have l₂ := (Prod.Lex.le_iff (i, b₁) (i,j)).mpr l₁
+          have l₃ := @lindenbaumSequenceMonotone t Δ (i,j) (i, b₁)  l₂
+          apply le_trans l₃
+          intros f h₃
+          sorry
+
+          
+  termination_by lindenbaumSequenceMonotone t Δ b => (b.fst, b.snd)
+
+def lindenbaumExtension (t : Th) (Δ : Ctx) : Ctx := {f | ∃n m : Nat, f ∈ lindenbaumSequence t Δ ⟨n, m⟩ }
 
 lemma lindenbaumExtensionExtends { t : Th } { Δ : Ctx } : t.val ⊆ lindenbaumExtension t Δ := by
   intros f h₁
